{
 "cells": [
  {
   "cell_type": "markdown",
   "metadata": {},
   "source": [
    "# Question 2.1\n",
    "\n",
    "## Part (a)\n",
    "\n",
    "For proving Abelian group, we need to prove the following properties:\n",
    "\n",
    "### Closure\n",
    "\n",
    "Consider two elements, $a$ and $b$ which are part of $R$\\\\{-1}, then:\n",
    "\n",
    "$$a*b = ab + a + b$$\n",
    "\n",
    "Since, $a$ and $b$ are real numbers, $ab$, $a$ and $b$ will also be real numbers, and thus, their sum will also be real. We only need to check if $a*b$ can result in -1.\n",
    "\n",
    "Let's assume that for $a$ and $b$ not equal to -1, $a*b$ is -1. Then:\n",
    "\n",
    "$$ab + a + b = -1$$\n",
    "\n",
    "$$a(b+1) + b = -1$$\n",
    "\n",
    "$$a(b+1) = -(b+1)$$\n",
    "\n",
    "$$a = -1$$ \n",
    "\n",
    "The above step can be performed, since, $b \\ne 1$\n",
    "\n",
    "But, we know that $a \\ne 1$, so, $ab + a + b \\ne 1$.\n",
    "\n",
    "Hence, we have proven the closure property.\n",
    "\n",
    "### Associativity\n",
    "\n",
    "\n",
    "Consider three elements, $a$, $b$ and $c$ which are part of $R$\\\\{-1}, then:\n",
    "\n",
    "$$a*(b*c) = a*(bc + b + c)$$\n",
    "\n",
    "$$a*(b*c) = a(bc + b + c) + a + (bc + b + c)$$\n",
    "\n",
    "$$a*(b*c) = abc + ab + ac + a + bc + b + c$$\n",
    "\n",
    "$$a*(b*c) = abc + ac + bc + c + ab + a + b$$\n",
    "\n",
    "$$a*(b*c) = (ab + a + b)c + (ab + a + b) + c$$\n",
    "\n",
    "$$a*(b*c) = (a*b)c + (a*b) + c$$\n",
    "\n",
    "$$a*(b*c) = (a*b)*c$$\n",
    "\n",
    "Hence, we have proven the associativity property.\n",
    "\n",
    "\n",
    "### Neutral Element\n",
    "\n",
    "Consider two elements, $a$ and $e$ which are part of $R$\\\\{-1}, such that:\n",
    "\n",
    "$a*e = a$ and $e*a = a$\n",
    "\n",
    "We need to check if such an element $e$ exists or not.\n",
    "\n",
    "$$a*e = ae + a + e$$\n",
    "\n",
    "$$a = ae + a + e$$\n",
    "\n",
    "$$ae + e = 0$$\n",
    "\n",
    "$$(a+1)e = 0$$\n",
    "\n",
    "Since, $a \\ne 1$\n",
    "\n",
    "$$e = 0$$\n",
    "\n",
    "We also know that {0} is a part of $R$\\\\{-1}, so, we have found that such an element exists. Now, let's verify if $e*a = a$ is true or not.\n",
    "\n",
    "$$e*a = ea + a + e$$\n",
    "\n",
    "$$a = ea + a + e$$\n",
    "\n",
    "$$ea + e = 0$$\n",
    "\n",
    "$$(a+1)e = 0$$\n",
    "\n",
    "$$e = 0$$\n",
    "\n",
    "We have reached at the same element.\n",
    "\n",
    "Hence, we have proved that a neutral element exists.\n",
    "\n",
    "\n",
    "### Inverse Element\n",
    "\n",
    "\n",
    "Consider two elements, $a$ and $b$, and the neutral element, $e$, all lying in $R$\\\\{-1}. We have to check if the following condition can be fulfilled for any $b$ or not, given $a$.\n",
    "\n",
    "$$a * b = e$$\n",
    "\n",
    "$$ab + a + b = e$$\n",
    "\n",
    "Since we know that $e = 0$\n",
    "\n",
    "$$ab + a + b = 0$$\n",
    "\n",
    "$$a(b+1) = -b$$\n",
    "\n",
    "Since $b \\ne 1$\n",
    "\n",
    "$$a = \\frac{-b}{b+1}$$\n",
    "\n",
    "For a real number $b$, the above $a$ will also be a real number. We need to check if $a$ can be -1 or not. Let's assume that $a = -1$, then,\n",
    "\n",
    "$$-1 = \\frac{-b}{b+1}$$\n",
    "\n",
    "$$b+1 = b$$\n",
    "\n",
    "$$1 = 0$$\n",
    "\n",
    "The above statement is clearly false, which means that $a \\ne -1$. Thus, $a$ also lies in $R$\\\\{-1}\n",
    "\n",
    "Hence, we have seen that for any $b$ lying in $R$\\\\{-1}, an inverse element $a = \\frac{-b}{b+1}$ lying in $R$\\\\{-1} also exists.\n",
    "\n",
    "\n",
    "### Commutativity\n",
    "\n",
    "Consider two elements $a$ and $b$ lying in $R$\\\\{-1}, then\n",
    "\n",
    "$$a * b = ab + a + b$$\n",
    "\n",
    "$$a * b = ba + b + a$$\n",
    "\n",
    "$$a * b = b * a$$\n",
    "\n",
    "This proves the commutative property as well.\n",
    "\n",
    "Since all the above properties hold true, we can $(R$\\\\{-1}, $*)$ is an Abelian group.\n",
    "\n",
    "\n",
    "## Part (b)\n",
    "\n",
    "$$3 * x * x = 15$$\n",
    "\n",
    "$$(3 * x) * x = 15$$\n",
    "\n",
    "$$(3x + x + 3) * x = 15$$\n",
    "\n",
    "$$(4x + 3) * x = 15$$\n",
    "\n",
    "$$(4x + 3)x + (4x + 3) + x = 15$$\n",
    "\n",
    "$$4x^2 + 3x + 4x + 3 + x = 15$$\n",
    "\n",
    "$$4x^2 + 8x + 3 = 15$$\n",
    "\n",
    "$$4x^2 + 8x - 12 = 0$$\n",
    "\n",
    "$$x^2 + 2x - 3 = 0$$\n",
    "\n",
    "$$(x-2)(x-1) = 0$$\n",
    "\n",
    "$$x = 2, x = 1$$"
   ]
  },
  {
   "cell_type": "markdown",
   "metadata": {},
   "source": [
    "# Question 2.2"
   ]
  }
 ],
 "metadata": {
  "kernelspec": {
   "display_name": "Python 3",
   "language": "python",
   "name": "python3"
  },
  "language_info": {
   "codemirror_mode": {
    "name": "ipython",
    "version": 3
   },
   "file_extension": ".py",
   "mimetype": "text/x-python",
   "name": "python",
   "nbconvert_exporter": "python",
   "pygments_lexer": "ipython3",
   "version": "3.7.1"
  }
 },
 "nbformat": 4,
 "nbformat_minor": 2
}
